TreeCode.thy
@@ -7,7 +7,6 @@ datatype tree_code =
   | TPushCon nat
   | TPushLam "tree_code list"
   | TApply
-  | TEnter
   | TReturn
   | TJump
 
@@ -19,12 +18,12 @@ datatype tree_code_state = TS "tclosure list" "tclosure list list" "tree_code li
 
 inductive evalt :: "tree_code_state \<Rightarrow> tree_code_state \<Rightarrow> bool" (infix "\<leadsto>\<^sub>t" 50) where
   evt_lookup [simp]: "lookup env x = Some v \<Longrightarrow> 
-    TS vs (env # envs) (TLookup x # cd) \<leadsto>\<^sub>t TS (v # vs) envs cd"
-| evt_pushcon [simp]: "TS vs (env # envs) (TPushCon k # cd) \<leadsto>\<^sub>t TS (TConst k # vs) envs cd"
-| evt_pushlam [simp]: "TS vs (env # envs) (TPushLam cd' # cd) \<leadsto>\<^sub>t TS (TLam env cd' # vs) envs cd"
+    TS vs (env # envs) (TLookup x # cd) \<leadsto>\<^sub>t TS (v # vs) (env # envs) cd"
+| evt_pushcon [simp]: "TS vs envs (TPushCon k # cd) \<leadsto>\<^sub>t TS (TConst k # vs) envs cd"
+| evt_pushlam [simp]: "TS vs (env # envs) (TPushLam cd' # cd) \<leadsto>\<^sub>t 
+    TS (TLam env cd' # vs) (env # envs) cd"
 | evt_apply [simp]: "TS (v # TLam env cd' # vs) envs (TApply # cd) \<leadsto>\<^sub>t 
     TS vs ((v # env) # envs) (cd' @ cd)"
-| evt_enter [simp]: "TS vs (env # envs) (TEnter # cd) \<leadsto>\<^sub>t TS vs (env # env # envs) cd"
 | evt_return [simp]: "TS vs (env # envs) (TReturn # cd) \<leadsto>\<^sub>t TS vs envs cd"
 | evt_jump [simp]: "TS (v # TLam env' cd' # vs) (env # envs) (TJump # cd) \<leadsto>\<^sub>t 
     TS vs ((v # env') # envs) (cd' @ cd)"
@@ -35,8 +34,8 @@ proof (induction \<Sigma> \<Sigma>' rule: evalt.induct)
   from evt_lookup(2, 1) show ?case 
     by (induction "TS vs (env # envs) (TLookup x # cd)" \<Sigma>'' rule: evalt.induct) simp_all 
 next
-  case (evt_pushcon vs env envs k cd)
-  thus ?case by (induction "TS vs (env # envs) (TPushCon k # cd)" \<Sigma>'' rule: evalt.induct) simp_all 
+  case (evt_pushcon vs envs k cd)
+  thus ?case by (induction "TS vs envs (TPushCon k # cd)" \<Sigma>'' rule: evalt.induct) simp_all 
 next
   case (evt_pushlam vs env envs cd' cd)
   thus ?case by (induction "TS vs (env # envs) (TPushLam cd' # cd)" \<Sigma>'' rule: evalt.induct) simp_all 
@@ -44,9 +43,6 @@ next
   case (evt_apply v env cd' vs envs cd)
   thus ?case 
     by (induction "TS (v # TLam env cd' # vs) envs (TApply # cd)" \<Sigma>'' rule: evalt.induct) simp_all 
-next
-  case (evt_enter vs env envs cd)
-  thus ?case by (induction "TS vs (env # envs) (TEnter # cd)" \<Sigma>'' rule: evalt.induct) simp_all 
 next
   case (evt_return vs env envs cd)
   thus ?case by (induction "TS vs (env # envs) (TReturn # cd)" \<Sigma>'' rule: evalt.induct) simp_all 
