HeapMemory.thy
@@ -11,19 +11,15 @@ datatype heap_state =
 
 inductive evalh :: "heap_state \<Rightarrow> heap_state \<Rightarrow> bool" (infix "\<leadsto>\<^sub>h" 50) where
   evh_lookup [simp]: "cd ! pc = BLookup x \<Longrightarrow> lookup env x = Some v \<Longrightarrow> 
-    HS h vs (env # envs) (Suc pc # pcs) cd \<leadsto>\<^sub>h HS h (v # vs) envs (pc # pcs) cd"
+    HS h vs (env # envs) (Suc pc # pcs) cd \<leadsto>\<^sub>h HS h (v # vs) (env # envs) (pc # pcs) cd"
 | evh_pushcon [simp]: "cd ! pc = BPushCon k \<Longrightarrow> halloc h (HConst k) = (h', v) \<Longrightarrow>
-    HS h vs (env # envs) (Suc pc # pcs) cd \<leadsto>\<^sub>h HS h' (v # vs) envs (pc # pcs) cd"
+    HS h vs envs (Suc pc # pcs) cd \<leadsto>\<^sub>h HS h' (v # vs) envs (pc # pcs) cd"
 | evh_pushlam [simp]: "cd ! pc = BPushLam pc' \<Longrightarrow> halloc h (HLam env pc') = (h', v) \<Longrightarrow>
-    HS h vs (env # envs) (Suc pc # pcs) cd \<leadsto>\<^sub>h HS h' (v # vs) envs (pc # pcs) cd"
-| evh_enter [simp]: "cd ! pc = BEnter \<Longrightarrow> 
-    HS h vs (env # envs) (Suc pc # pcs) cd \<leadsto>\<^sub>h HS h vs (env # env # envs) (pc # pcs) cd"
+    HS h vs (env # envs) (Suc pc # pcs) cd \<leadsto>\<^sub>h HS h' (v # vs) (env # envs) (pc # pcs) cd"
 | evh_apply [simp]: "cd ! pc = BApply \<Longrightarrow> hlookup h v2 = HLam env pc' \<Longrightarrow>
     HS h (v1 # v2 # vs) envs (Suc pc # pcs) cd \<leadsto>\<^sub>h
       HS h vs ((v1 # env) # envs) (pc' # pc # pcs) cd"
-| evh_return [simp]: "cd ! pc = BReturn_Old \<Longrightarrow> 
-    HS h vs envs (Suc pc # pcs) cd \<leadsto>\<^sub>h HS h vs envs pcs cd"
-| evh_returnb [simp]: "cd ! pc = BReturn \<Longrightarrow> 
+| evh_return [simp]: "cd ! pc = BReturn \<Longrightarrow> 
     HS h vs (env # envs) (Suc pc # pcs) cd \<leadsto>\<^sub>h HS h vs envs pcs cd"
 | evh_jump [simp]: "cd ! pc = BJump \<Longrightarrow> hlookup h v2 = HLam env' pc' \<Longrightarrow>
     HS h (v1 # v2 # vs) (env # envs) (Suc pc # pcs) cd \<leadsto>\<^sub>h 
@@ -35,16 +31,12 @@ proof (induction \<Sigma> \<Sigma>' rule: evalh.induct)
   from evh_lookup(3, 1, 2) show ?case 
     by (induction "HS h vs (env # envs) (Suc pc # pcs) cd" \<Sigma>'' rule: evalh.induct) simp_all 
 next
-  case (evh_pushcon cd pc k h h' v vs env envs pcs)
+  case (evh_pushcon cd pc k h h' v vs envs pcs)
   from evh_pushcon(3, 1, 2) show ?case 
-    by (induction "HS h vs (env # envs) (Suc pc # pcs) cd" \<Sigma>'' rule: evalh.induct) simp_all 
+    by (induction "HS h vs envs (Suc pc # pcs) cd" \<Sigma>'' rule: evalh.induct) simp_all 
 next
   case (evh_pushlam cd pc pc' h env h' v vs envs pcs)
   from evh_pushlam(3, 1, 2) show ?case 
-    by (induction "HS h vs (env # envs) (Suc pc # pcs) cd" \<Sigma>'' rule: evalh.induct) simp_all 
-next
-  case (evh_enter cd pc h vs env envs pcs)
-  from evh_enter(2, 1) show ?case 
     by (induction "HS h vs (env # envs) (Suc pc # pcs) cd" \<Sigma>'' rule: evalh.induct) simp_all 
 next
   case (evh_apply cd pc h v2 env pc' v1 vs envs pcs)
@@ -52,12 +44,8 @@ next
     by (induction "HS h (v1 # v2 # vs) envs (Suc pc # pcs) cd" \<Sigma>'' rule: evalh.induct) 
        simp_all 
 next
-  case (evh_return cd pc h vs envs pcs)
+  case (evh_return cd pc h vs env envs pcs)
   from evh_return(2, 1) show ?case 
-    by (induction "HS h vs envs (Suc pc # pcs) cd" \<Sigma>'' rule: evalh.induct) simp_all 
-next
-  case (evh_returnb cd pc h vs env envs pcs)
-  from evh_returnb(2, 1) show ?case 
     by (induction "HS h vs (env # envs) (Suc pc # pcs) cd" \<Sigma>'' rule: evalh.induct) simp_all 
 next
   case (evh_jump cd pc h v2 env' pc' v1 vs env envs pcs)
