Iteration.thy
@@ -9,7 +9,7 @@ inductive iter :: "('a \<Rightarrow> 'a \<Rightarrow> bool) \<Rightarrow> 'a \<R
 lemma iter_append: "iter f a b \<Longrightarrow> iter f b c \<Longrightarrow> iter f a c"
   by (induction a b rule: iter.induct) simp_all
 
-lemma [simp]: "iter f a b \<Longrightarrow> f b c \<Longrightarrow> iter f a c"
+lemma iter_step_after [simp]: "iter f a b \<Longrightarrow> f b c \<Longrightarrow> iter f a c"
   by (induction a b rule: iter.induct) simp_all
 
 end
