MemoryFlattening.thy
@@ -53,16 +53,16 @@ lemma get_closure_flatten [simp]: "hsplay splay_closure h = (h', mp) \<Longright
 
 theorem completef [simp]: "\<Sigma>\<^sub>h \<leadsto>\<^sub>h \<Sigma>\<^sub>h' \<Longrightarrow> heap_structured \<Sigma>\<^sub>h \<Longrightarrow> flatten \<Sigma>\<^sub>h \<leadsto>\<^sub>f flatten \<Sigma>\<^sub>h'"
 proof (induction \<Sigma>\<^sub>h \<Sigma>\<^sub>h' rule: evalh.induct)
-  case (evh_pushcon cd pc k h h' v vs env envs pcs)
-  hence S: "stack_contains h vs \<and> stack_contains h env \<and> env_contains h envs" by simp
+  case (evh_pushcon cd pc k h h' v vs envs pcs)
+  hence S: "stack_contains h vs \<and> env_contains h envs" by simp
   obtain h\<^sub>1 mp where H1: "hsplay splay_closure h = (h\<^sub>1, mp)" by fastforce
   obtain h\<^sub>2 y where H2: "halloc_list h\<^sub>1 [0, k] = (h\<^sub>2, y)" by fastforce
   with evh_pushcon H1 have H3: "hsplay splay_closure h' = (h\<^sub>2, mp(v := y))" by simp
-  from evh_pushcon H2 have "FS h\<^sub>1 (map mp vs) (map mp env # map (map mp) envs) (Suc pc # pcs) cd \<leadsto>\<^sub>f 
+  from evh_pushcon H2 have "FS h\<^sub>1 (map mp vs) (map (map mp) envs) (Suc pc # pcs) cd \<leadsto>\<^sub>f 
     FS h\<^sub>2 (y # map mp vs) (map (map mp) envs) (pc # pcs) cd" by simp
   moreover from evh_pushcon S H1 have "map (mp(v := y)) vs = map mp vs" by fastforce
   moreover from evh_pushcon S H1 have "map (map (mp(v := y))) envs = map (map mp) envs" by fastforce
-  ultimately have "FS h\<^sub>1 (map mp vs) (map mp env # map (map mp) envs) (Suc pc # pcs) cd \<leadsto>\<^sub>f
+  ultimately have "FS h\<^sub>1 (map mp vs) (map (map mp) envs) (Suc pc # pcs) cd \<leadsto>\<^sub>f
     FS h\<^sub>2 (y # map (mp(v := y)) vs) (map (map (mp(v := y))) envs) (pc # pcs) cd" by metis
   with H1 H3 show ?case by simp
 next
@@ -74,11 +74,13 @@ next
   with evh_pushlam H1 have H3: "hsplay splay_closure h' = (h\<^sub>2, mp(v := y))" 
     by (simp del: halloc_list.simps)
   from evh_pushlam H2 have "FS h\<^sub>1 (map mp vs) (map mp env # map (map mp) envs) (Suc pc # pcs) cd \<leadsto>\<^sub>f 
-    FS h\<^sub>2 (y # map mp vs) (map (map mp) envs) (pc # pcs) cd" by simp
+    FS h\<^sub>2 (y # map mp vs) (map mp env # map (map mp) envs) (pc # pcs) cd" by simp
   moreover from evh_pushlam S H1 have "map (mp(v := y)) vs = map mp vs" by fastforce
+  moreover from evh_pushlam S H1 have "map (mp(v := y)) env = map mp env" by fastforce
   moreover from evh_pushlam S H1 have "map (map (mp(v := y))) envs = map (map mp) envs" by fastforce
   ultimately have "FS h\<^sub>1 (map mp vs) (map mp env # map (map mp) envs) (Suc pc # pcs) cd \<leadsto>\<^sub>f
-    FS h\<^sub>2 (y # map (mp(v := y)) vs) (map (map (mp(v := y))) envs) (pc # pcs) cd" by metis
+    FS h\<^sub>2 (y # map (mp(v := y)) vs) (map (mp(v := y)) env # map (map (mp(v := y))) envs) 
+      (pc # pcs) cd" by metis
   with H1 H3 show ?case by simp
 qed (simp_all del: get_closure.simps split: prod.splits)
 
